src/absyn/syntax.fs
@@ -172,7 +172,9 @@ type qualifier =
   | Logic
   | Discriminator of lident                          (* discriminator for a datacon l *)
   | Projector of lident * either<btvdef, bvvdef>     (* projector for datacon l's argument 'a or x *)
-  | Logic_record
+  | RecordType of list<ident>                        (* unmangled field names *)
+  | RecordConstructor of list<ident>                 (* unmangled field names *)
+  | ExceptionConstructor
   | Effect 
  
 type monad_abbrev = {
@@ -208,7 +210,7 @@ type monad_decl = {
 and sigelt =
   | Sig_tycon          of lident * list<tparam> * knd * list<lident> * list<lident> * list<qualifier> * Range.range (* bool is for a prop, list<lident> identifies mutuals, second list<lident> are all the constructors *)
   | Sig_typ_abbrev     of lident * list<tparam> * knd * typ * list<qualifier> * Range.range 
-  | Sig_datacon        of lident * typ * lident * Range.range  (* second lident is the name of the type this constructs *)
+  | Sig_datacon        of lident * typ * lident * list<qualifier> * Range.range  (* second lident is the name of the type this constructs *)
   | Sig_val_decl       of lident * typ * list<qualifier> * Range.range 
   | Sig_assume         of lident * formula * list<qualifier> * Range.range 
   | Sig_let            of letbindings * Range.range 
